platform/Depl/PtsToEntail.v
@@ -172,8 +172,8 @@ Inductive lhs_remains (p : list pred) := .
 Definition entail (lhs rhs : ppred) :=
   let lhs' := normalize (ppredX lhs) in
   let rhs' := normalize (ppredX rhs) in
-    match cancel nil lhs' rhs' with
-      | Success lhs'' P =>
+    match cancel nil nil lhs' rhs' with
+      | Success _ lhs'' P =>
         match lhs'' with
           | nil => ProveThis P
           | _ => Failed (lhs_remains lhs'')
@@ -204,13 +204,15 @@ Theorem entail_correct : forall lhs rhs bl br P,
   -> pimpl lhs rhs.
 Proof.
   unfold entail; intros.
-  case_eq (cancel nil (normalize (ppredX lhs)) (normalize (ppredX rhs))); intros.
+  case_eq (cancel nil nil (normalize (ppredX lhs)) (normalize (ppredX rhs))); intros.
   Focus 2.
   rewrite H5 in *; discriminate.
   rewrite H5 in *.
   destruct NewLhs; try discriminate.
   injection H; clear H; intros; subst.
-  specialize (cancel_sound nil fo_empty _ hE S _ _ _ _ H5); intuition.
+  assert (Hfe : forall x, In x (@nil string) -> ~In x nil)
+    by (simpl; tauto).
+  specialize (cancel_sound nil nil fo_empty _ hE S _ _ _ _ _ Hfe H5); intuition.
   rewrite <- app_nil_end in *.
   match type of H6 with
     | ?P -> _ => assert P by eauto; intuition
